git/fgdorais/GMLAlgebra/GMLAlgebra/AddMul.lean
@@ -1,0 +1,187 @@
+import GMLAlgebra.Signatures
+import GMLAlgebra.Identities
+import GMLAlgebra.UnitalRig
+import GMLAlgebra.UnitalRing
+import GMLAlgebra.UnitalSemiring
+
+namespace Algebra
+variable (α)
+  [HAdd α α α] [Neg α] [OfNat α (nat_lit 0)]
+  [HMul α α α] [Inv α] [OfNat α (nat_lit 1)]
+
+def addSemigroupSig : SemigroupSig α where
+  op := (.+.)
+
+unif_hint (t : SemigroupSig α) where
+  t =?= addSemigroupSig α ⊢ t.op =?= (.+.)
+
+def addMonoidSig : MonoidSig α where
+  toSemigroupSig := addSemigroupSig α
+  id := 0
+
+unif_hint (t : MonoidSig α) where
+  t =?= addMonoidSig α ⊢ t.toSemigroupSig =?= addSemigroupSig α
+
+unif_hint (t : MonoidSig α) where
+  t =?= addMonoidSig α ⊢ t.id =?= 0
+
+def addGroupSig : GroupSig α where
+  toMonoidSig := addMonoidSig α
+  inv := (-.)
+
+unif_hint (t : GroupSig α) where
+  t =?= addGroupSig α ⊢ t.toMonoidSig =?= addMonoidSig α
+
+unif_hint (t : GroupSig α) where
+  t =?= addGroupSig α ⊢ t.inv =?= (-.)
+
+def mulSemigroupSig : SemigroupSig α where
+  op := (.*.)
+
+unif_hint (t : SemigroupSig α) where
+  t =?= mulSemigroupSig α ⊢ t.op =?= (.*.)
+
+def mulMonoidSig : MonoidSig α where
+  toSemigroupSig := mulSemigroupSig α
+  id := 1
+
+unif_hint (t : MonoidSig α) where
+  t =?= mulMonoidSig α ⊢ t.toSemigroupSig =?= mulSemigroupSig α
+
+unif_hint (t : MonoidSig α) where
+  t =?= mulMonoidSig α ⊢ t.id =?= 1
+
+def mulGroupSig : GroupSig α where
+  toMonoidSig := mulMonoidSig α
+  inv := (.⁻¹)
+
+unif_hint (t : GroupSig α) where
+  t =?= mulGroupSig α ⊢ t.toMonoidSig =?= mulMonoidSig α
+
+unif_hint (t : GroupSig α) where
+  t =?= mulGroupSig α ⊢ t.inv =?= (.⁻¹)
+
+def addMulSemiringSig : SemiringSig α where
+  add := (.+.)
+  mul := (.*.)
+
+unif_hint (t : SemiringSig α) where
+  t =?= addMulSemiringSig α ⊢ t.toAddSemigroupSig =?= addSemigroupSig α
+
+unif_hint (t : SemiringSig α) where
+  t =?= addMulSemiringSig α ⊢ t.toMulSemigroupSig =?= mulSemigroupSig α
+
+unif_hint (t : SemiringSig α) where
+  t =?= addMulSemiringSig α ⊢ t.add =?= (.+.)
+
+unif_hint (t : SemiringSig α) where
+  t =?= addMulSemiringSig α ⊢ t.mul =?= (.*.)
+
+def addMulRigSig : RigSig α where
+  toSemiringSig := addMulSemiringSig α
+  zero := 0
+
+unif_hint (t : RigSig α) where
+  t =?= addMulRigSig α ⊢ t.toAddMonoidSig =?= addMonoidSig α
+
+unif_hint (t : RigSig α) where
+  t =?= addMulRigSig α ⊢ t.toSemiringSig =?= addMulSemiringSig α
+
+unif_hint (t : RigSig α) where
+  t =?= addMulRigSig α ⊢ t.zero =?= 0
+
+def addMulRingSig : RingSig α where
+  toRigSig := addMulRigSig α
+  neg := (-.)
+
+unif_hint (t : RingSig α) where
+  t =?= addMulRingSig α ⊢ t.toAddGroupSig =?= addGroupSig α
+
+unif_hint (t : RingSig α) where
+  t =?= addMulRingSig α ⊢ t.toRigSig =?= addMulRigSig α
+
+unif_hint (t : RingSig α) where
+  t =?= addMulRingSig α ⊢ t.neg =?= (-.)
+
+def addMulUnitalSemiringSig : UnitalSemiringSig α where
+  toSemiringSig := addMulSemiringSig α
+  one := 1
+
+unif_hint (t : UnitalSemiringSig α) where
+  t =?= addMulUnitalSemiringSig α ⊢ t.toMulMonoidSig =?= mulMonoidSig α
+
+unif_hint (t : UnitalSemiringSig α) where
+  t =?= addMulUnitalSemiringSig α ⊢ t.toSemiringSig =?= addMulSemiringSig α
+
+unif_hint (t : UnitalSemiringSig α) where
+  t =?= addMulUnitalSemiringSig α ⊢ t.one =?= 1
+
+def addMulUnitalRigSig : UnitalRigSig α where
+  toRigSig := addMulRigSig α
+  one := 1
+
+unif_hint (t : UnitalRigSig α) where
+  t =?= addMulUnitalRigSig α ⊢ t.toUnitalSemiringSig.toMulMonoidSig =?= mulMonoidSig α
+
+unif_hint (t : UnitalRigSig α) where
+  t =?= addMulUnitalRigSig α ⊢ t.toUnitalSemiringSig =?= addMulUnitalSemiringSig α
+
+unif_hint (t : UnitalRigSig α) where
+  t =?= addMulUnitalRigSig α ⊢ t.toSemiringSig =?= addMulSemiringSig α
+
+unif_hint (t : UnitalRigSig α) where
+  t =?= addMulUnitalRigSig α ⊢ t.one =?= 1
+
+def addMulUnitalRingSig : UnitalRingSig α where
+  toRingSig := addMulRingSig α
+  one := 1
+
+unif_hint (t : UnitalRingSig α) where
+  t =?= addMulUnitalRingSig α ⊢ t.toMulMonoidSig =?= mulMonoidSig α
+
+unif_hint (t : UnitalRingSig α) where
+  t =?= addMulUnitalRingSig α ⊢ t.toUnitalSemiringSig =?= addMulUnitalSemiringSig α
+
+unif_hint (t : UnitalRingSig α) where
+  t =?= addMulUnitalRingSig α ⊢ t.toUnitalRigSig =?= addMulUnitalRigSig α
+
+unif_hint (t : UnitalRingSig α) where
+  t =?= addMulUnitalRingSig α ⊢ t.toSemiringSig =?= addMulSemiringSig α
+
+unif_hint (t : UnitalRingSig α) where
+  t =?= addMulUnitalRingSig α ⊢ t.one =?= 1
+
+end Algebra
+
+section instances
+open Algebra
+
+instance Pos.instUnitalCommSemiring : UnitalCommSemiring (addMulUnitalSemiringSig Pos) where
+  add_assoc := Pos.add_assoc
+  add_comm := Pos.add_comm
+  mul_assoc := Pos.mul_assoc
+  mul_comm := Pos.mul_comm
+  mul_right_id := Pos.mul_one
+  mul_right_distrib := Pos.right_distrib
+
+instance Nat.instUnitalCommRig : UnitalCommRig (addMulUnitalRigSig Nat) where
+  add_assoc := Nat.add_assoc
+  add_comm := Nat.add_comm
+  add_right_id := Nat.add_zero
+  mul_assoc := Nat.mul_assoc
+  mul_comm := Nat.mul_comm
+  mul_right_id := Nat.mul_one
+  mul_right_distrib := Nat.right_distrib
+  mul_right_zero := Nat.mul_zero
+
+instance Int.instUnitalCommRing : UnitalCommRing (addMulUnitalRingSig Int) where
+  add_assoc := Int.add_assoc
+  add_comm := Int.add_comm
+  add_right_id := Int.add_zero
+  add_right_inv := Int.add_neg
+  mul_assoc := Int.mul_assoc
+  mul_comm := Int.mul_comm
+  mul_right_id := Int.mul_one
+  mul_right_distrib := Int.add_mul
+
+end instances
